staged/LibFmap.v
@@ -1,49 +1,83 @@
-
 From SLF Require Import LibCore.
 From SLF Require Export LibSepFmap.
 
 Module Fmap := LibSepFmap.
 
-Lemma fmap_disjoint_indom : forall (A B: Type) (h1 h2 : fmap A B) x,
-  disjoint h1 h2 -> indom h1 x -> ~ indom h2 x.
+Lemma fmap_disjoint_indom :
+  forall (A B : Type)
+         (h1 h2 : fmap A B)
+         (x : A),
+    disjoint h1 h2 -> indom h1 x -> ~ indom h2 x.
 Proof.
-  unfold not; intros.
-  apply (disjoint_inv_not_indom_both H H0).
-  auto.
+  unfold not.
+  exact disjoint_inv_not_indom_both.
 Qed.
 
-Lemma fmap_indom_empty : forall A B (k:A),
-  ~ indom (@empty A B) k.
-Proof.
-  intros.
-  unfold not; intros.
-  hnf in H.
-  unfold empty in H.
-  apply H.
-  simpl.
-  reflexivity.
-Qed.
+Lemma fmap_not_indom_empty :
+  forall (A B : Type)
+         (x : A),
+    ~ indom (@empty A B) x.
+Proof. auto. Qed.
 
-Lemma fmap_read_update : forall A B {IB:Inhab B} (k:A) (v:B) m,
-  read (update m k v) k = v.
+Search (Fmap.read).
+
+Lemma fmap_read_update :
+  forall (A B : Type)
+         {IB : Inhab B}
+         (h : fmap A B)
+         (x : A)
+         (v : B),
+    read (update h x v) x = v.
 Proof.
   intros.
   unfold update.
-  rewrite read_union_l.
-  apply read_single.
-  apply indom_single.
+  rewrite -> (read_union_l h (indom_single x v)).
+  exact (read_single x v).
 Qed.
 
 #[global]
 Hint Rewrite fmap_read_update : rew_fmap rew_fmap_for_fmap_eq.
 
-Lemma fmap_not_indom_of_neq : forall (A B:Type) (a b:A) (v:B),
-  a <> b -> ~ Fmap.indom (Fmap.single a v) b.
+Lemma fmap_neq_not_indom :
+  forall (A B : Type)
+         (x y : A)
+         (v : B),
+    x <> y ->
+    ~ Fmap.indom (Fmap.single x v) y.
+Proof.
+  unfold not.
+  intros A B x y v H_neq H_indom.
+  rewrite -> (indom_single_eq x y v) in H_indom.
+  contradiction.
+Qed.
+
+Lemma fmap_single_union_single_eq_single :
+  forall (A B : Type)
+         (x : A)
+         (v w : B),
+    single x v \+ single x w = single x v.
+Proof.
+  intros A B x v w.
+  apply fmap_extens.
+  intro y.
+  unfold union.
+  unfold map_union.
+  simpl.
+  destruct (classicT _); reflexivity.
+Qed.
+
+Lemma fmap_update_update_eq_update :
+  forall (A B : Type)
+         (h : fmap A B)
+         (x : A)
+         (v w : B),
+    update (update h x v) x w = update h x w.
 Proof.
   intros.
-  unfold not. intros.
-  rewrite (Fmap.indom_single_eq a b v) in H0.
-  contradiction.
+  unfold update.
+  rewrite <- union_assoc.
+  rewrite -> fmap_single_union_single_eq_single.
+  reflexivity.
 Qed.
 
 Ltac solve_trivial_not_indom :=
